fix sndop issues and add strcture proof

theory/Assembler.thy
@@ -5,12 +5,9 @@ imports
   rBPFCommType rBPFSyntax
 begin
 
-definition insn :: "u8 \<Rightarrow> i64 \<Rightarrow> i64 \<Rightarrow> i64 \<Rightarrow> i64 \<Rightarrow> ebpf_binary option" where
+definition insn :: "u8 \<Rightarrow> u4 \<Rightarrow> u4 \<Rightarrow> i16 \<Rightarrow> i32 \<Rightarrow> ebpf_binary option" where
 "insn opc dst src off imm = 
-  ( if dst <s 0 \<or> 10 <s dst then None else
-    if src <s 0 \<or> 10 <s src then None else
-    if off <s (-32768) \<or> 32767 <s off then None else
-    if imm <s (-2147483648) \<or> 2147483647 <s imm then None else
+  ( if 10 < dst \<or> 10 < src then None else
       Some \<lparr> bpf_opc = opc,
             bpf_dst = (ucast dst),
             bpf_src = (ucast src),
@@ -23,460 +20,197 @@ fun ldx_chunk2opcode :: "chunk \<Rightarrow> u8" where
 "ldx_chunk2opcode SWord = 0x61" |
 "ldx_chunk2opcode DWord = 0x79"
 
-fun st_chunk2opcode :: "chunk \<Rightarrow> snd_op \<Rightarrow> u8" where
-"st_chunk2opcode Byte (SOImm _) = 0x72" |
-"st_chunk2opcode Byte (SOReg _) = 0x73" |
-"st_chunk2opcode HalfWord (SOImm _) = 0x6a" |
-"st_chunk2opcode HalfWord (SOReg _) = 0x6b" |
-"st_chunk2opcode SWord (SOImm _) = 0x62" |
-"st_chunk2opcode SWord (SOReg _) = 0x63" |
-"st_chunk2opcode DWord (SOImm _) = 0x7a" |
-"st_chunk2opcode DWord (SOReg _) = 0x7b"
+fun st_chunk2opcode_imm :: "chunk \<Rightarrow> u8" where
+"st_chunk2opcode_imm Byte = 0x72" |
+"st_chunk2opcode_imm HalfWord  = 0x6a" |
+"st_chunk2opcode_imm SWord = 0x62" |
+"st_chunk2opcode_imm DWord  = 0x7a"
 
-fun alu2opcode :: "binop \<Rightarrow> snd_op \<Rightarrow> u8" where
-"alu2opcode BPF_ADD (SOImm _) = 0x04" |
-"alu2opcode BPF_ADD (SOReg _) = 0x0c" |
-"alu2opcode BPF_SUB (SOImm _) = 0x14" |
-"alu2opcode BPF_SUB (SOReg _) = 0x1c" |
-"alu2opcode BPF_MUL (SOImm _) = 0x24" |
-"alu2opcode BPF_MUL (SOReg _) = 0x2c" |
-"alu2opcode BPF_DIV (SOImm _) = 0x34" |
-"alu2opcode BPF_DIV (SOReg _) = 0x3c" |
-"alu2opcode BPF_OR  (SOImm _) = 0x44" |
-"alu2opcode BPF_OR  (SOReg _) = 0x4c" |
-"alu2opcode BPF_AND (SOImm _) = 0x54" |
-"alu2opcode BPF_AND (SOReg _) = 0x5c" |
-"alu2opcode BPF_LSH (SOImm _) = 0x64" |
-"alu2opcode BPF_LSH (SOReg _) = 0x6c" |
-"alu2opcode BPF_RSH (SOImm _) = 0x74" |
-"alu2opcode BPF_RSH (SOReg _) = 0x7c" |
-"alu2opcode BPF_MOD (SOImm _) = 0x94" |
-"alu2opcode BPF_MOD (SOReg _) = 0x9c" |
-"alu2opcode BPF_XOR (SOImm _) = 0xa4" |
-"alu2opcode BPF_XOR (SOReg _) = 0xac" |
-"alu2opcode BPF_MOV (SOImm _) = 0xb4" |
-"alu2opcode BPF_MOV (SOReg _) = 0xbc" |
-"alu2opcode BPF_ARSH (SOImm _) = 0xc4" |
-"alu2opcode BPF_ARSH (SOReg _) = 0xcc"
+fun st_chunk2opcode_reg :: "chunk \<Rightarrow> u8" where
+"st_chunk2opcode_reg Byte = 0x73" |
+"st_chunk2opcode_reg HalfWord  = 0x6b" |
+"st_chunk2opcode_reg SWord = 0x63" |
+"st_chunk2opcode_reg DWord = 0x7b"
 
-fun alu642opcode :: "binop \<Rightarrow> snd_op \<Rightarrow> u8" where
-"alu642opcode BPF_ADD (SOImm _) = 0x07" |
-"alu642opcode BPF_ADD (SOReg _) = 0x0f" |
-"alu642opcode BPF_SUB (SOImm _) = 0x17" |
-"alu642opcode BPF_SUB (SOReg _) = 0x1f" |
-"alu642opcode BPF_MUL (SOImm _) = 0x27" |
-"alu642opcode BPF_MUL (SOReg _) = 0x2f" |
-"alu642opcode BPF_DIV (SOImm _) = 0x37" |
-"alu642opcode BPF_DIV (SOReg _) = 0x3f" |
-"alu642opcode BPF_OR  (SOImm _) = 0x47" |
-"alu642opcode BPF_OR  (SOReg _) = 0x4f" |
-"alu642opcode BPF_AND (SOImm _) = 0x57" |
-"alu642opcode BPF_AND (SOReg _) = 0x5f" |
-"alu642opcode BPF_LSH (SOImm _) = 0x67" |
-"alu642opcode BPF_LSH (SOReg _) = 0x6f" |
-"alu642opcode BPF_RSH (SOImm _) = 0x77" |
-"alu642opcode BPF_RSH (SOReg _) = 0x7f" |
-"alu642opcode BPF_MOD (SOImm _) = 0x97" |
-"alu642opcode BPF_MOD (SOReg _) = 0x9f" |
-"alu642opcode BPF_XOR (SOImm _) = 0xa7" |
-"alu642opcode BPF_XOR (SOReg _) = 0xaf" |
-"alu642opcode BPF_MOV (SOImm _) = 0xb7" |
-"alu642opcode BPF_MOV (SOReg _) = 0xbf" |
-"alu642opcode BPF_ARSH (SOImm _) = 0xc7" |
-"alu642opcode BPF_ARSH (SOReg _) = 0xcf"
-
-fun snd_op2i64 :: "snd_op \<Rightarrow> i64" where
-"snd_op2i64 (SOReg ir) = (bpf_ireg2i64 ir)" |
-"snd_op2i64 (SOImm im) = (scast im)"
-
-fun pqr2opcode :: "pqrop \<Rightarrow> snd_op \<Rightarrow> u8" where
-"pqr2opcode BPF_LMUL (SOImm _) = 0x86" |
-"pqr2opcode BPF_LMUL (SOReg _) = 0x8e" |
-"pqr2opcode BPF_UDIV (SOImm _) = 0x46" |
-"pqr2opcode BPF_UDIV (SOReg _) = 0x4e" |
-"pqr2opcode BPF_UREM (SOImm _) = 0x66" |
-"pqr2opcode BPF_UREM (SOReg _) = 0x6e" |
-"pqr2opcode BPF_SDIV (SOImm _) = 0xc6" |
-"pqr2opcode BPF_SDIV (SOReg _) = 0xce" |
-"pqr2opcode BPF_SREM (SOImm _) = 0xe6" |
-"pqr2opcode BPF_SREM (SOReg _) = 0xee"
-
-fun pqr642opcode :: "pqrop \<Rightarrow> snd_op \<Rightarrow> u8" where
-"pqr642opcode BPF_LMUL (SOImm _) = 0x96" |
-"pqr642opcode BPF_LMUL (SOReg _) = 0x9e" |
-"pqr642opcode BPF_UDIV (SOImm _) = 0x56" |
-"pqr642opcode BPF_UDIV (SOReg _) = 0x5e" |
-"pqr642opcode BPF_UREM (SOImm _) = 0x76" |
-"pqr642opcode BPF_UREM (SOReg _) = 0x7e" |
-"pqr642opcode BPF_SDIV (SOImm _) = 0xd6" |
-"pqr642opcode BPF_SDIV (SOReg _) = 0xde" |
-"pqr642opcode BPF_SREM (SOImm _) = 0xf6" |
-"pqr642opcode BPF_SREM (SOReg _) = 0xfe"
-
-fun pqr22opcode :: "pqrop2 \<Rightarrow> snd_op \<Rightarrow> u8" where
-"pqr22opcode BPF_UHMUL (SOImm _) = 0x36" |
-"pqr22opcode BPF_UHMUL (SOReg _) = 0x3e" |
-"pqr22opcode BPF_SHMUL (SOImm _) = 0xb6" |
-"pqr22opcode BPF_SHMUL (SOReg _) = 0xbe"
+fun alu2opcode_imm :: "binop \<Rightarrow> u8" where
+"alu2opcode_imm BPF_ADD  = 0x04" |
+"alu2opcode_imm BPF_SUB  = 0x14" |
+"alu2opcode_imm BPF_MUL  = 0x24" |
+"alu2opcode_imm BPF_DIV  = 0x34" |
+"alu2opcode_imm BPF_OR   = 0x44" |
+"alu2opcode_imm BPF_AND  = 0x54" |
+"alu2opcode_imm BPF_LSH  = 0x64" |
+"alu2opcode_imm BPF_RSH  = 0x74" |
+"alu2opcode_imm BPF_MOD  = 0x94" |
+"alu2opcode_imm BPF_XOR  = 0xa4" |
+"alu2opcode_imm BPF_MOV  = 0xb4" |
+"alu2opcode_imm BPF_ARSH  = 0xc4"
 
 
-fun condition2opcode :: "condition \<Rightarrow> snd_op \<Rightarrow> u8" where
-"condition2opcode Eq  (SOImm _) = 0x15" |
-"condition2opcode Eq  (SOReg _) = 0x1d" |
-"condition2opcode Gt  (SOImm _) = 0x25" |
-"condition2opcode Gt  (SOReg _) = 0x2d" |
-"condition2opcode Ge  (SOImm _) = 0x35" |
-"condition2opcode Ge  (SOReg _) = 0x3d" |
-"condition2opcode Lt  (SOImm _) = 0xa5" |
-"condition2opcode Lt  (SOReg _) = 0xad" |
-"condition2opcode Le  (SOImm _) = 0xb5" |
-"condition2opcode Le  (SOReg _) = 0xbd" |
-"condition2opcode SEt (SOImm _) = 0x45" |
-"condition2opcode SEt (SOReg _) = 0x4d" |
-"condition2opcode Ne  (SOImm _) = 0x55" |
-"condition2opcode Ne  (SOReg _) = 0x5d" |
-"condition2opcode SGt (SOImm _) = 0x65" |
-"condition2opcode SGt (SOReg _) = 0x6d" |
-"condition2opcode SGe (SOImm _) = 0x75" |
-"condition2opcode SGe (SOReg _) = 0x7d" |
-"condition2opcode SLt (SOImm _) = 0xc5" |
-"condition2opcode SLt (SOReg _) = 0xcd" |
-"condition2opcode SLe (SOImm _) = 0xd5" |
-"condition2opcode SLe (SOReg _) = 0xdd"
+fun alu2opcode_reg :: "binop \<Rightarrow> u8" where
+"alu2opcode_reg BPF_ADD  = 0x0c" |
+"alu2opcode_reg BPF_SUB  = 0x1c" |
+"alu2opcode_reg BPF_MUL  = 0x2c" |
+"alu2opcode_reg BPF_DIV  = 0x3c" |
+"alu2opcode_reg BPF_OR   = 0x4c" |
+"alu2opcode_reg BPF_AND  = 0x5c" |
+"alu2opcode_reg BPF_LSH  = 0x6c" |
+"alu2opcode_reg BPF_RSH  = 0x7c" |
+"alu2opcode_reg BPF_MOD  = 0x9c" |
+"alu2opcode_reg BPF_XOR  = 0xac" |
+"alu2opcode_reg BPF_MOV  = 0xbc" |
+"alu2opcode_reg BPF_ARSH = 0xcc"
+
+
+fun alu642opcode_imm :: "binop \<Rightarrow> u8" where
+"alu642opcode_imm BPF_ADD  = 0x07" |
+"alu642opcode_imm BPF_SUB  = 0x17" |
+"alu642opcode_imm BPF_MUL  = 0x27" |
+"alu642opcode_imm BPF_DIV  = 0x37" |
+"alu642opcode_imm BPF_OR   = 0x47" |
+"alu642opcode_imm BPF_AND  = 0x57" |
+"alu642opcode_imm BPF_LSH  = 0x67" |
+"alu642opcode_imm BPF_RSH  = 0x77" |
+"alu642opcode_imm BPF_MOD  = 0x97" |
+"alu642opcode_imm BPF_XOR  = 0xa7" |
+"alu642opcode_imm BPF_MOV  = 0xb7" |
+"alu642opcode_imm BPF_ARSH  = 0xc7"
+
+
+fun alu642opcode_reg :: "binop \<Rightarrow> u8" where
+"alu642opcode_reg BPF_ADD  = 0x0f" |
+"alu642opcode_reg BPF_SUB  = 0x1f" |
+"alu642opcode_reg BPF_MUL  = 0x2f" |
+"alu642opcode_reg BPF_DIV  = 0x3f" |
+"alu642opcode_reg BPF_OR   = 0x4f" |
+"alu642opcode_reg BPF_AND  = 0x5f" |
+"alu642opcode_reg BPF_LSH  = 0x6f" |
+"alu642opcode_reg BPF_RSH  = 0x7f" |
+"alu642opcode_reg BPF_MOD  = 0x9f" |
+"alu642opcode_reg BPF_XOR  = 0xaf" |
+"alu642opcode_reg BPF_MOV  = 0xbf" |
+"alu642opcode_reg BPF_ARSH = 0xcf"
+
+fun pqr2opcode_imm :: "pqrop \<Rightarrow> u8" where
+"pqr2opcode_imm BPF_LMUL  = 0x86" |
+"pqr2opcode_imm BPF_UDIV  = 0x46" |
+"pqr2opcode_imm BPF_UREM  = 0x66" |
+"pqr2opcode_imm BPF_SDIV  = 0xc6" |
+"pqr2opcode_imm BPF_SREM  = 0xe6"
+
+fun pqr2opcode_reg :: "pqrop \<Rightarrow> u8" where
+"pqr2opcode_reg BPF_LMUL  = 0x8e" |
+"pqr2opcode_reg BPF_UDIV  = 0x4e" |
+"pqr2opcode_reg BPF_UREM  = 0x6e" |
+"pqr2opcode_reg BPF_SDIV  = 0xce" |
+"pqr2opcode_reg BPF_SREM  = 0xee"
+
+fun pqr642opcode_imm :: "pqrop \<Rightarrow> u8" where
+"pqr642opcode_imm BPF_LMUL  = 0x96" |
+"pqr642opcode_imm BPF_UDIV  = 0x56" |
+"pqr642opcode_imm BPF_UREM  = 0x76" |
+"pqr642opcode_imm BPF_SDIV  = 0xd6" |
+"pqr642opcode_imm BPF_SREM  = 0xf6"
+
+fun pqr642opcode_reg :: "pqrop \<Rightarrow> u8" where
+"pqr642opcode_reg BPF_LMUL  = 0x9e" |
+"pqr642opcode_reg BPF_UDIV  = 0x5e" |
+"pqr642opcode_reg BPF_UREM  = 0x7e" |
+"pqr642opcode_reg BPF_SDIV  = 0xde" |
+"pqr642opcode_reg BPF_SREM  = 0xfe"
+
+fun pqr22opcode_imm :: "pqrop2 \<Rightarrow> u8" where
+"pqr22opcode_imm BPF_UHMUL  = 0x36" |
+"pqr22opcode_imm BPF_SHMUL  = 0xb6"
+
+fun pqr22opcode_reg :: "pqrop2 \<Rightarrow> u8" where
+"pqr22opcode_reg BPF_UHMUL  = 0x3e" |
+"pqr22opcode_reg BPF_SHMUL  = 0xbe"
+
+
+fun condition2opcode_imm :: "condition \<Rightarrow> u8" where
+"condition2opcode_imm Eq   = 0x15" |
+"condition2opcode_imm Gt   = 0x25" |
+"condition2opcode_imm Ge   = 0x35" |
+"condition2opcode_imm Lt   = 0xa5" |
+"condition2opcode_imm Le   = 0xb5" |
+"condition2opcode_imm SEt  = 0x45" |
+"condition2opcode_imm Ne   = 0x55" |
+"condition2opcode_imm SGt  = 0x65" |
+"condition2opcode_imm SGe  = 0x75" |
+"condition2opcode_imm SLt  = 0xc5" |
+"condition2opcode_imm SLe  = 0xd5"
+
+fun condition2opcode_reg :: "condition \<Rightarrow> u8" where
+"condition2opcode_reg Eq   = 0x1d" |
+"condition2opcode_reg Gt   = 0x2d" |
+"condition2opcode_reg Ge   = 0x3d" |
+"condition2opcode_reg Lt   = 0xad" |
+"condition2opcode_reg Le   = 0xbd" |
+"condition2opcode_reg SEt  = 0x4d" |
+"condition2opcode_reg Ne   = 0x5d" |
+"condition2opcode_reg SGt  = 0x6d" |
+"condition2opcode_reg SGe  = 0x7d" |
+"condition2opcode_reg SLt  = 0xcd" |
+"condition2opcode_reg SLe  = 0xdd"
 
 fun assemble_one_instruction :: "bpf_instruction \<Rightarrow> ebpf_binary option" where
 "assemble_one_instruction (BPF_LD_IMM dst i1 i2) =
-  insn 0x18 (bpf_ireg2i64 dst) 0 0 (scast i1)" |
+  insn 0x18 (bpf_ireg2u4 dst) 0 0 i1" |
 "assemble_one_instruction (BPF_LDX ck dst src off) =
-  insn (ldx_chunk2opcode ck) (bpf_ireg2i64 dst) (bpf_ireg2i64 src) (scast off) 0" |
-"assemble_one_instruction (BPF_ST ck dst src off) =
-  insn (st_chunk2opcode ck src) (bpf_ireg2i64 dst) (snd_op2i64 src) (scast off) 0" |
+  insn (ldx_chunk2opcode ck) (bpf_ireg2u4 dst) (bpf_ireg2u4 src) off 0" |
+"assemble_one_instruction (BPF_ST ck dst (SOReg ir) off) =
+  insn (st_chunk2opcode_reg ck) (bpf_ireg2u4 dst) (bpf_ireg2u4 ir) off 0" |
+"assemble_one_instruction (BPF_ST ck dst (SOImm im) off) =
+  insn (st_chunk2opcode_imm ck) (bpf_ireg2u4 dst) 0 off im" |
   
 "assemble_one_instruction (BPF_NEG32_REG dst) =
-  insn 0x84 (bpf_ireg2i64 dst) 0 0 0" |
+  insn 0x84 (bpf_ireg2u4 dst) 0 0 0" |
 "assemble_one_instruction (BPF_NEG64_REG dst) =
-  insn 0x87 (bpf_ireg2i64 dst) 0 0 0" |
+  insn 0x87 (bpf_ireg2u4 dst) 0 0 0" |
   
-"assemble_one_instruction (BPF_ALU bop dst src) =
-  insn (alu2opcode bop src) (bpf_ireg2i64 dst) (snd_op2i64 src) 0 0" |
+"assemble_one_instruction (BPF_ALU bop dst (SOReg ir)) =
+  insn (alu2opcode_reg bop) (bpf_ireg2u4 dst) (bpf_ireg2u4 ir) 0 0" |
+"assemble_one_instruction (BPF_ALU bop dst (SOImm im)) =
+  insn (alu2opcode_imm bop) (bpf_ireg2u4 dst) 0 0 im" |
 "assemble_one_instruction (BPF_LE dst imm) =
-  insn 0xd4 (bpf_ireg2i64 dst) 0 0 (scast imm)" |
+  insn 0xd4 (bpf_ireg2u4 dst) 0 0 imm" |
 "assemble_one_instruction (BPF_BE dst imm) =
-  insn 0xdc (bpf_ireg2i64 dst) 0 0 (scast imm)" |
+  insn 0xdc (bpf_ireg2u4 dst) 0 0 imm" |
   
-"assemble_one_instruction (BPF_ALU64 bop dst src) =
-  insn (alu642opcode bop src) (bpf_ireg2i64 dst) (snd_op2i64 src) 0 0" |
+"assemble_one_instruction (BPF_ALU64 bop dst (SOReg ir)) =
+  insn (alu642opcode_reg bop) (bpf_ireg2u4 dst) (bpf_ireg2u4 ir) 0 0" |
+"assemble_one_instruction (BPF_ALU64 bop dst (SOImm im)) =
+  insn (alu642opcode_imm bop) (bpf_ireg2u4 dst) 0 0 im" |
 "assemble_one_instruction (BPF_HOR64_IMM dst imm) =
-  insn 0xf7 (bpf_ireg2i64 dst) 0 0 (scast imm)" |
+  insn 0xf7 (bpf_ireg2u4 dst) 0 0 imm" |
   
-"assemble_one_instruction (BPF_PQR pop dst src) =
-  insn (pqr2opcode pop src) (bpf_ireg2i64 dst) (snd_op2i64 src) 0 0" |
-"assemble_one_instruction (BPF_PQR64 pop dst src) =
-  insn (pqr642opcode pop src) (bpf_ireg2i64 dst) (snd_op2i64 src) 0 0" |
-"assemble_one_instruction (BPF_PQR2 pop dst src) =
-  insn (pqr22opcode pop src) (bpf_ireg2i64 dst) (snd_op2i64 src) 0 0" |
+"assemble_one_instruction (BPF_PQR pop dst (SOReg ir)) =
+  insn (pqr2opcode_reg pop) (bpf_ireg2u4 dst) (bpf_ireg2u4 ir) 0 0" |
+"assemble_one_instruction (BPF_PQR pop dst (SOImm im)) =
+  insn (pqr2opcode_imm pop) (bpf_ireg2u4 dst) 0 0 im" |
+"assemble_one_instruction (BPF_PQR64 pop dst (SOReg ir)) =
+  insn (pqr642opcode_reg pop) (bpf_ireg2u4 dst) (bpf_ireg2u4 ir) 0 0" |
+"assemble_one_instruction (BPF_PQR64 pop dst (SOImm im)) =
+  insn (pqr642opcode_imm pop) (bpf_ireg2u4 dst) 0 0 im" |
+"assemble_one_instruction (BPF_PQR2 pop dst (SOReg ir)) =
+  insn (pqr22opcode_reg pop) (bpf_ireg2u4 dst) (bpf_ireg2u4 ir) 0 0" |
+"assemble_one_instruction (BPF_PQR2 pop dst (SOImm im)) =
+  insn (pqr22opcode_imm pop) (bpf_ireg2u4 dst) 0 0 im" |
   
 "assemble_one_instruction (BPF_JA off) =
-  insn 0x5 0 0 (scast off) 0" |
-"assemble_one_instruction (BPF_JUMP cop dst src off) =
-  insn (condition2opcode cop src) (bpf_ireg2i64 dst) (snd_op2i64 src) (scast off) 0" |
+  insn 0x5 0 0 off 0" |
+"assemble_one_instruction (BPF_JUMP cop dst (SOReg ir) off) =
+  insn (condition2opcode_reg cop) (bpf_ireg2u4 dst) (bpf_ireg2u4 ir) off 0" |
+"assemble_one_instruction (BPF_JUMP cop dst (SOImm im) off) =
+  insn (condition2opcode_imm cop) (bpf_ireg2u4 dst) 0 off im" |
   
 "assemble_one_instruction (BPF_CALL_REG src imm) =
-  insn 0x8d 0 (bpf_ireg2i64 src) 0 (scast imm)" |
+  insn 0x8d 0 (bpf_ireg2u4 src) 0 imm" |
 "assemble_one_instruction (BPF_CALL_IMM src imm) =
-  insn 0x85 0 (bpf_ireg2i64 src) 0 (scast imm)" |
+  insn 0x85 0 (bpf_ireg2u4 src) 0 imm" |
   
 "assemble_one_instruction BPF_EXIT = insn 0x95 0 0 0 0"
-
-
-  (*
-definition st_chunk2opcode :: "chunk \<Rightarrow> snd_op \<Rightarrow> u8" where
-"st_chunk2opcode ck sop = (
-  case ck of
-  Byte \<Rightarrow> (
-    case sop of 
-    (SOImm _) \<Rightarrow> 0x72 |
-    (SOReg _) \<Rightarrow> 0x73) |
-  HalfWord \<Rightarrow> (
-    case sop of 
-    (SOImm _) \<Rightarrow> 0x6a |
-    (SOReg _) \<Rightarrow> 0x6b) |
-  SWord \<Rightarrow> (
-    case sop of 
-    (SOImm _) \<Rightarrow> 0x62 |
-    (SOReg _) \<Rightarrow> 0x63) |
-  DWord \<Rightarrow> (
-    case sop of 
-    (SOImm _) \<Rightarrow> 0x7a |
-    (SOReg _) \<Rightarrow> 0x7b))"
-
-definition alu2opcode :: "binop \<Rightarrow> snd_op \<Rightarrow> u8" where
-"alu2opcode bop sop = (
-  case bop of 
-  BPF_ADD \<Rightarrow> (
-    case sop of 
-    (SOImm _) \<Rightarrow> 0x04 |
-    (SOReg _) \<Rightarrow> 0x0c) |
-  BPF_SUB \<Rightarrow> (
-    case sop of 
-    (SOImm _) \<Rightarrow> 0x14 |
-    (SOReg _) \<Rightarrow> 0x1c) |
-  BPF_MUL \<Rightarrow> (
-    case sop of 
-    (SOImm _) \<Rightarrow> 0x24 |
-    (SOReg _) \<Rightarrow> 0x2c) |
-  BPF_DIV \<Rightarrow> (
-    case sop of 
-    (SOImm _) \<Rightarrow> 0x34 |
-    (SOReg _) \<Rightarrow> 0x3c) |
-  BPF_OR \<Rightarrow> (
-    case sop of 
-    (SOImm _) \<Rightarrow> 0x44 |
-    (SOReg _) \<Rightarrow> 0x4c) |
-  BPF_AND \<Rightarrow> (
-    case sop of 
-    (SOImm _) \<Rightarrow> 0x54 |
-    (SOReg _) \<Rightarrow> 0x5c) |
-  BPF_LSH \<Rightarrow> (
-    case sop of 
-    (SOImm _) \<Rightarrow> 0x64 |
-    (SOReg _) \<Rightarrow> 0x6c) |
-  BPF_RSH \<Rightarrow> (
-    case sop of 
-    (SOImm _) \<Rightarrow> 0x74 |
-    (SOReg _) \<Rightarrow> 0x7c) |
-  BPF_MOD \<Rightarrow> (
-    case sop of 
-    (SOImm _) \<Rightarrow> 0x94 |
-    (SOReg _) \<Rightarrow> 0x9c) |
-  BPF_XOR \<Rightarrow> (
-    case sop of 
-    (SOImm _) \<Rightarrow> 0xa4 |
-    (SOReg _) \<Rightarrow> 0xac) |
-  BPF_MOV \<Rightarrow> (
-    case sop of 
-    (SOImm _) \<Rightarrow> 0xb4 |
-    (SOReg _) \<Rightarrow> 0xbc) |
-  BPF_ARSH \<Rightarrow> (
-    case sop of 
-    (SOImm _) \<Rightarrow> 0xc4 |
-    (SOReg _) \<Rightarrow> 0xcc)
- )"
-
-definition alu642opcode :: "binop \<Rightarrow> snd_op \<Rightarrow> u8" where
-"alu642opcode bop sop = (
-  case bop of 
-  BPF_ADD \<Rightarrow> (
-    case sop of 
-    (SOImm _) \<Rightarrow> 0x07 |
-    (SOReg _) \<Rightarrow> 0x0f) |
-  BPF_SUB \<Rightarrow> (
-    case sop of 
-    (SOImm _) \<Rightarrow> 0x17 |
-    (SOReg _) \<Rightarrow> 0x1f) |
-  BPF_MUL \<Rightarrow> (
-    case sop of 
-    (SOImm _) \<Rightarrow> 0x27 |
-    (SOReg _) \<Rightarrow> 0x2f) |
-  BPF_DIV \<Rightarrow> (
-    case sop of 
-    (SOImm _) \<Rightarrow> 0x37 |
-    (SOReg _) \<Rightarrow> 0x3f) |
-  BPF_OR \<Rightarrow> (
-    case sop of 
-    (SOImm _) \<Rightarrow> 0x47 |
-    (SOReg _) \<Rightarrow> 0x4f) |
-  BPF_AND \<Rightarrow> (
-    case sop of 
-    (SOImm _) \<Rightarrow> 0x57 |
-    (SOReg _) \<Rightarrow> 0x5f) |
-  BPF_LSH \<Rightarrow> (
-    case sop of 
-    (SOImm _) \<Rightarrow> 0x67 |
-    (SOReg _) \<Rightarrow> 0x6f) |
-  BPF_RSH \<Rightarrow> (
-    case sop of 
-    (SOImm _) \<Rightarrow> 0x77 |
-    (SOReg _) \<Rightarrow> 0x7f) |
-  BPF_MOD \<Rightarrow> (
-    case sop of 
-    (SOImm _) \<Rightarrow> 0x97 |
-    (SOReg _) \<Rightarrow> 0x9f) |
-  BPF_XOR \<Rightarrow> (
-    case sop of 
-    (SOImm _) \<Rightarrow> 0xa7 |
-    (SOReg _) \<Rightarrow> 0xaf) |
-  BPF_MOV \<Rightarrow> (
-    case sop of 
-    (SOImm _) \<Rightarrow> 0xb7 |
-    (SOReg _) \<Rightarrow> 0xbf) |
-  BPF_ARSH \<Rightarrow> (
-    case sop of 
-    (SOImm _) \<Rightarrow> 0xc7 |
-    (SOReg _) \<Rightarrow> 0xcf)
- )"
-
-
-definition snd_op2i64 :: "snd_op \<Rightarrow> i64" where
-"snd_op2i64 sop = (
- case sop of
- SOReg ir \<Rightarrow> bpf_ireg2i64 ir |
- SOImm im \<Rightarrow> scast im)"
-
-definition pqr2opcode :: "pqrop \<Rightarrow> snd_op \<Rightarrow> u8" where
-"pqr2opcode pop sop = (
-  case pop of
-  BPF_LMUL \<Rightarrow> (
-    case sop of
-    SOImm _ \<Rightarrow> 0x86 |
-    SOReg _ \<Rightarrow> 0x8e) |
-  BPF_UDIV  \<Rightarrow> (
-    case sop of
-    SOImm _ \<Rightarrow> 0x46 |
-    SOReg _ \<Rightarrow> 0x4e) |
-  BPF_UREM  \<Rightarrow> (
-    case sop of
-    SOImm _ \<Rightarrow> 0x66 |
-    SOReg _ \<Rightarrow> 0x6e) |
-  BPF_SDIV  \<Rightarrow> (
-    case sop of
-    SOImm _ \<Rightarrow> 0xc6 |
-    SOReg _ \<Rightarrow> 0xce) |
-  BPF_SREM  \<Rightarrow> (
-    case sop of
-    SOImm _ \<Rightarrow> 0xe6 |
-    SOReg _ \<Rightarrow> 0xee))"
-
-definition pqr642opcode :: "pqrop \<Rightarrow> snd_op \<Rightarrow> u8" where
-"pqr642opcode pop sop = (
-  case pop of
-  BPF_LMUL \<Rightarrow> (
-    case sop of
-    SOImm _ \<Rightarrow> 0x96 |
-    SOReg _ \<Rightarrow> 0x9e) |
-  BPF_UDIV \<Rightarrow> (
-    case sop of
-    SOImm _ \<Rightarrow> 0x56 |
-    SOReg _ \<Rightarrow> 0x5e) |
-  BPF_UREM \<Rightarrow> (
-    case sop of
-    SOImm _ \<Rightarrow> 0x76 |
-    SOReg _ \<Rightarrow> 0x7e) |
-  BPF_SDIV \<Rightarrow> (
-    case sop of
-    SOImm _ \<Rightarrow> 0xd6 |
-    SOReg _ \<Rightarrow> 0xde) |
-  BPF_SREM \<Rightarrow> (
-    case sop of
-    SOImm _ \<Rightarrow> 0xf6 |
-    SOReg _ \<Rightarrow> 0xfe))"
-
-definition pqr22opcode :: "pqrop2 \<Rightarrow> snd_op \<Rightarrow> u8" where
-"pqr22opcode pop sop = (
-  case pop of
-  BPF_UHMUL \<Rightarrow> (
-    case sop of
-    SOImm _ \<Rightarrow> 0x36 |
-    SOReg _ \<Rightarrow> 0x3e) |
-  BPF_SHMUL \<Rightarrow> (
-    case sop of
-    SOImm _ \<Rightarrow> 0xb6 |
-    SOReg _ \<Rightarrow> 0xbe))"
-
-
-definition condition2opcode :: "condition \<Rightarrow> snd_op \<Rightarrow> u8" where
-"condition2opcode cop sop = (
-  case cop of
-  Eq \<Rightarrow> (
-    case sop of
-    SOImm _ \<Rightarrow> 0x15 |
-    SOReg _ \<Rightarrow> 0x1d) |
-  Gt \<Rightarrow> (
-    case sop of
-    SOImm _ \<Rightarrow> 0x25 |
-    SOReg _ \<Rightarrow> 0x2d) |
-  Ge \<Rightarrow> (
-    case sop of
-    SOImm _ \<Rightarrow> 0x35 |
-    SOReg _ \<Rightarrow> 0x3d) |
-  Lt \<Rightarrow> (
-    case sop of
-    SOImm _ \<Rightarrow> 0xa5 |
-    SOReg _ \<Rightarrow> 0xad) |
-  Le \<Rightarrow> (
-    case sop of
-    SOImm _ \<Rightarrow> 0xb5 |
-    SOReg _ \<Rightarrow> 0xbd) |
-  SEt \<Rightarrow> (
-    case sop of
-    SOImm _ \<Rightarrow> 0x45 |
-    SOReg _ \<Rightarrow> 0x4d) |
-  Ne \<Rightarrow> (
-    case sop of
-    SOImm _ \<Rightarrow> 0x55 |
-    SOReg _ \<Rightarrow> 0x5d) |
-  SGt \<Rightarrow> (
-    case sop of
-    SOImm _ \<Rightarrow> 0x65 |
-    SOReg _ \<Rightarrow> 0x6d) |
-  SGe \<Rightarrow> (
-    case sop of
-    SOImm _ \<Rightarrow> 0x75 |
-    SOReg _ \<Rightarrow> 0x7d) |
-  SLt \<Rightarrow> (
-    case sop of
-    SOImm _ \<Rightarrow> 0xc5 |
-    SOReg _ \<Rightarrow> 0xcd) |
-  SLe \<Rightarrow> (
-    case sop of
-    SOImm _ \<Rightarrow> 0xd5 |
-    SOReg _ \<Rightarrow> 0xdd))"
- 
-definition assemble_one_instruction :: "bpf_instruction \<Rightarrow> ebpf_binary option" where
-"assemble_one_instruction ins = (
-  case ins of
-  BPF_LD_IMM dst i1 i2 \<Rightarrow>
-    insn 0x18 (bpf_ireg2i64 dst) 0 0 (scast i1) |
-  BPF_LDX ck dst src off \<Rightarrow>
-    insn (ldx_chunk2opcode ck) (bpf_ireg2i64 dst) (bpf_ireg2i64 src) (scast off) 0 |
-  BPF_ST ck dst src off \<Rightarrow>
-    insn (st_chunk2opcode ck src) (bpf_ireg2i64 dst) (snd_op2i64 src) (scast off) 0 |
-  
-  BPF_NEG32_REG dst \<Rightarrow>
-    insn 0x84 (bpf_ireg2i64 dst) 0 0 0 |
-  BPF_NEG64_REG dst \<Rightarrow>
-    insn 0x87 (bpf_ireg2i64 dst) 0 0 0 |
-  
-  BPF_ALU bop dst src \<Rightarrow>
-    insn (alu2opcode bop src) (bpf_ireg2i64 dst) (snd_op2i64 src) 0 0 |
-  BPF_LE dst imm \<Rightarrow>
-    insn 0xd4 (bpf_ireg2i64 dst) 0 0 (scast imm) |
-  BPF_BE dst imm \<Rightarrow>
-    insn 0xdc (bpf_ireg2i64 dst) 0 0 (scast imm) |
-  
-  BPF_ALU64 bop dst src \<Rightarrow>
-    insn (alu642opcode bop src) (bpf_ireg2i64 dst) (snd_op2i64 src) 0 0 |
-  BPF_HOR64_IMM dst imm \<Rightarrow>
-    insn 0xf7 (bpf_ireg2i64 dst) 0 0 (scast imm) |
-  
-  BPF_PQR pop dst src \<Rightarrow>
-    insn (pqr2opcode pop src) (bpf_ireg2i64 dst) (snd_op2i64 src) 0 0 |
-  BPF_PQR64 pop dst src \<Rightarrow>
-    insn (pqr642opcode pop src) (bpf_ireg2i64 dst) (snd_op2i64 src) 0 0 |
-  BPF_PQR2 pop dst src \<Rightarrow>
-    insn (pqr22opcode pop src) (bpf_ireg2i64 dst) (snd_op2i64 src) 0 0 |
-  
-  BPF_JA off \<Rightarrow>
-    insn 0x5 0 0 (scast off) 0 |
-  BPF_JUMP cop dst src off \<Rightarrow>
-    insn (condition2opcode cop src) (bpf_ireg2i64 dst) (snd_op2i64 src) (scast off) 0 |
-  
-  BPF_CALL_REG src imm \<Rightarrow>
-    insn 0x8d 0 (bpf_ireg2i64 src) 0 (scast imm) |
-  BPF_CALL_IMM src imm \<Rightarrow>
-    insn 0x85 0 (bpf_ireg2i64 src) 0 (scast imm) |
-  
-  BPF_EXIT \<Rightarrow> insn 0x95 0 0 0 0)" *)
 
 fun assemble :: "ebpf_asm \<Rightarrow> ebpf_bin option" where
 "assemble [] = Some []" |
@@ -489,7 +223,7 @@ fun assemble :: "ebpf_asm \<Rightarrow> ebpf_bin option" where
     Some tl_i \<Rightarrow> (
       case h of
       BPF_LD_IMM dst i1 i2 \<Rightarrow> (
-        case (insn 0 0 0 0 (scast i2)) of
+        case (insn 0 0 0 0 i2) of
         None \<Rightarrow> None |
         Some h_i2 \<Rightarrow> Some (h_i#h_i2#tl_i))|
        _ \<Rightarrow> Some (h_i#tl_i) )) )"
