theory/Consistency.thy
@@ -11,45 +11,19 @@ apply (unfold u4_to_bpf_ireg_def)
 apply auto
 done
 
-lemma u4_breg_i64 [simp]: "u4_to_bpf_ireg (bpf_dst x1) = Some aa \<Longrightarrow> (bpf_ireg2i64 aa) = (ucast (bpf_dst x1))"
-apply (unfold u4_to_bpf_ireg_def)
-apply (cases "bpf_dst x1 = 0")
-apply auto
-apply (cases "bpf_dst x1 = 1")
-apply auto
-apply (cases "bpf_dst x1 = 2")
-apply auto
-apply (cases "bpf_dst x1 = 3")
-apply auto
-apply (cases "bpf_dst x1 = 4")
-apply auto
-apply (cases "bpf_dst x1 = 5")
-apply auto
-apply (cases "bpf_dst x1 = 6")
-apply auto
-apply (cases "bpf_dst x1 = 7")
-apply auto
-apply (cases "bpf_dst x1 = 8")
-apply auto
-apply (cases "bpf_dst x1 = 9")
-apply auto
-apply (cases "bpf_dst x1 = 10")
-apply auto
-done
+declare if_split_asm [split] (**r register the lemma into split  *)
 
-lemma  bpf_ireg_i64_same [simp]: "u4_to_bpf_ireg (ucast (bpf_ireg2i64 x1)) = Some x1"
-apply (cases "x1", simp add: u4_to_bpf_ireg_def)
-apply (simp add: u4_to_bpf_ireg_def)
-apply (simp add: u4_to_bpf_ireg_def)
-apply (simp add: u4_to_bpf_ireg_def)
-apply (simp add: u4_to_bpf_ireg_def)
-apply (simp add: u4_to_bpf_ireg_def)
-apply (simp add: u4_to_bpf_ireg_def)
-apply (simp add: u4_to_bpf_ireg_def)
-apply (simp add: u4_to_bpf_ireg_def)
-apply (simp add: u4_to_bpf_ireg_def)
-apply (simp add: u4_to_bpf_ireg_def)
-done
+lemma u4_breg_i64 [simp]: "u4_to_bpf_ireg (bpf_dst x1) = Some aa \<Longrightarrow> (bpf_ireg2u4 aa) = (ucast (bpf_dst x1))"
+  by (unfold u4_to_bpf_ireg_def, auto) (**r simp add: split: if_split_asm *)
+(**r auto/simpl loads `split` *)
+
+
+lemma  bpf_ireg_i64_same [simp]: "u4_to_bpf_ireg (bpf_ireg2u4 x1) = Some x1"
+  by (cases "x1"; auto simp add: u4_to_bpf_ireg_def)
+(**r auto apply to all goals, simp only apply for the first one *)
+
+lemma bpf_ireg2u4_range [simp]: "0 \<le> bpf_ireg2u4 x2 \<and> bpf_ireg2u4 x2 \<le> 10"
+  by (cases x2; auto)
 
 lemma bpf_opc_simp[simp]:  "(bpf_opc
                  \<lparr>bpf_opc = x1,
@@ -81,196 +55,264 @@ lemma bpf_imm_simp[simp]:  "(bpf_imm
                     bpf_src = x3,
                     bpf_off = x4, bpf_imm = x5\<rparr> = x5)" by fastforce
 
+(*
+lemma scast_scast_id:
+  "scast (scast x :: ('a::len) signed word) = (x :: 'a word)"
+  "scast (scast y :: ('a::len) word) = (y :: 'a signed word)"
+  by (auto simp: is_up scast_up_scast_id)
+
+declare scast_scast_id[simp del]
+
+lemma "scast (scast x12::i32) = (x12::u32) "
+  apply (rule scast_scast_id(1))
+  
+  by (auto simp add: scast_scast_id) *)
 
 lemma assemble_disassemble_consistency: "assemble l_asm = Some l_bin \<Longrightarrow> disassemble l_bin = Some l_asm"
-apply (induction l_asm arbitrary: l_bin)
-apply simp
-apply simp+ 
-subgoal for x1 l_asm
+(*
+proof (induction l_asm arbitrary: l_bin)
+case Nil
+then show ?case by force
+next
+case (Cons x1 l_asm)
+then show ?case
+proof -
 
-apply (cases "assemble_one_instruction x1")
-apply auto
+assume IH: "(\<And>l_bin. assemble l_asm = Some l_bin \<Longrightarrow> disassemble l_bin = Some l_asm)"
+assume Hx1: "assemble (x1 # l_asm) = Some l_bin"
 
-apply (cases "assemble l_asm")
-apply auto
+from Hx1 have "(
+    case (assemble_one_instruction x1) of
+      None \<Rightarrow> None |
+      Some h_i \<Rightarrow> (
+        case (assemble l_asm) of
+        None \<Rightarrow> None |
+        Some tl_i \<Rightarrow> (
+          case x1 of
+          BPF_LD_IMM dst i1 i2 \<Rightarrow> (
+            case (insn 0 0 0 0 (scast i2)) of
+            None \<Rightarrow> None |
+            Some h_i2 \<Rightarrow> Some (h_i#h_i2#tl_i))|
+           _ \<Rightarrow> Some (h_i#tl_i) )) ) = Some l_bin" by simp
 
-subgoal for a aa
-apply (cases "x1", auto simp: insn_def) (**r , auto split: option.split *)
+thm Hx1 *)
 
-subgoal for x11 x12 x13
+  apply (induction l_asm arbitrary: l_bin)
+  subgoal
+    apply simp
+    done
+  subgoal for x1 l_asm
+    apply simp+ 
+    apply (cases "assemble_one_instruction x1", auto)
+    apply (cases "assemble l_asm", auto)
+    subgoal for a aa
+      apply (cases "x1", auto simp add: insn_def) (**r , auto split: option.split *)
+        (**r LD_IMM *)
+      subgoal for x11 x12 x13
+        apply (unfold disassemble_lddw_def, auto)   
+        done
 
-apply (cases "SCAST(32 signed \<rightarrow> 64 signed) x13
-             <s 0xFFFFFFFF80000000 \<or>
-             0x7FFFFFFF <s SCAST(32 signed \<rightarrow> 64 signed) x13")
-apply auto
+        (**r LDX + LD_IMM *)
+      subgoal for x21 x22 x23 x24
+        apply (cases x21, auto)
+        done
 
-apply (unfold disassemble_lddw_def)
-apply auto
-apply (cases "bpf_ireg2i64 x11 <s 0 \<or> 0xA <s bpf_ireg2i64 x11", auto)
-apply (cases " SCAST(32 signed \<rightarrow> 64 signed) x12
-        <s 0xFFFFFFFF80000000 \<or>
-        0x7FFFFFFF <s SCAST(32 signed \<rightarrow> 64 signed) x12", auto)
+        (**r LDX - LD_IMM *)
+      subgoal for x1 x2 x3 x4
+        apply (unfold disassemble_one_instruction_def)
+        apply (cases x1, auto)
+        done
 
-apply (cases "bpf_ireg2i64 x11 <s 0 \<or> 0xA <s bpf_ireg2i64 x11", auto)
-apply (cases " SCAST(32 signed \<rightarrow> 64 signed) x12
-        <s 0xFFFFFFFF80000000 \<or>
-        0x7FFFFFFF <s SCAST(32 signed \<rightarrow> 64 signed) x12", auto)
-.
+(**r ST + LD_IMM *)
+      subgoal for x31 x32 x33 x34
+        apply (cases x33, auto)
+        apply (unfold insn_def, cases x31, auto)
+        apply (cases x31, auto)
+        done
 
-subgoal for x21 x22 x23 x24
-apply (unfold disassemble_lddw_def)
-apply (cases "bpf_ireg2i64 x22 <s 0 \<or> 0xA <s bpf_ireg2i64 x22", auto)
-apply (cases "bpf_ireg2i64 x23 <s 0 \<or> 0xA <s bpf_ireg2i64 x23", auto)
-apply (cases " SCAST(16 signed \<rightarrow> 64 signed) x24 <s 0xFFFFFFFFFFFF8000 \<or> 0x7FFF <s SCAST(16 signed \<rightarrow> 64 signed) x24", auto)
+(**r ST - LD_IMM *)
+      subgoal for x31 x32 x33 x34
+        apply (unfold disassemble_one_instruction_def)
+        apply (cases x33, auto)
+        subgoal  
+          apply (unfold insn_def, cases x31, auto)  
+          done
+        subgoal for x1
+          apply (unfold insn_def, cases x31, auto)
+          done
+        subgoal for x1
+          apply (unfold insn_def, cases x31, auto)
+          done
+        subgoal for x1
+          apply (unfold insn_def, cases x31, auto)
+          done
+        done
 
-apply (cases x21, auto)
-.
+(**r ALU + LD_IMM *)
+      subgoal for x1 x2 x3
+        apply (cases x3; auto)
+         apply (unfold insn_def, cases x1; auto)
+        apply (unfold insn_def, cases x1; auto)
+        done
 
-subgoal for x1 x2 x3 x4
-apply (cases "bpf_ireg2i64 x2 <s 0 \<or> 0xA <s bpf_ireg2i64 x2")
-apply auto
+(**r ALU - LD_IMM *)
+      subgoal for x1 x2 x3
+        apply (unfold disassemble_one_instruction_def)
+        apply (cases x3, auto)
+        subgoal  
+          apply (unfold insn_def, cases x1, auto)                                        
+          done
+        subgoal  
+          apply (unfold insn_def, cases x1, auto)                                        
+          done
+        subgoal  
+          apply (unfold insn_def, cases x1, auto)                                        
+          done
+        subgoal  
+          apply (unfold insn_def, cases x1, auto)                                        
+          done
+        done  
 
-apply (cases "bpf_ireg2i64 x3 <s 0 \<or> 0xA <s bpf_ireg2i64 x3")
-apply auto
+(**r NEG32 *)
+      subgoal for x1
+        apply (unfold disassemble_one_instruction_def, auto)
+        done  
 
-apply (cases "SCAST(16 signed \<rightarrow> 64 signed) x4 <s 0xFFFFFFFFFFFF8000 \<or> 0x7FFF <s SCAST(16 signed \<rightarrow> 64 signed) x4")
-apply auto
+(**r LE *)
+      subgoal for x1 x2
+        apply (unfold disassemble_one_instruction_def, auto)
+        done  
 
-apply (cases x1)
-apply auto
+(**r BE *)
+      subgoal for x1 x2
+        apply (unfold disassemble_one_instruction_def, auto)
+        done  
+(**r ALU64 + LD_IMM *)
+      subgoal for x1 x2 x3
+        apply (cases x3; auto)
+        apply (unfold insn_def, cases x1; auto)
+        apply (unfold insn_def, cases x1; auto)
+        done
 
-apply (unfold disassemble_one_instruction_def, auto)
-.
+(**r ALU64 - LD_IMM  *)
+      subgoal for x1 x2 x3
+        apply (unfold disassemble_one_instruction_def)
+        apply (cases x3, auto)
+        subgoal  
+          apply (unfold insn_def, cases x1, auto)                                        
+          done
+        subgoal  
+          apply (unfold insn_def, cases x1, auto)                                        
+          done
+        subgoal  
+          apply (unfold insn_def, cases x1, auto)                                        
+          done
+        subgoal  
+          apply (unfold insn_def, cases x1, auto)                                        
+          done
+        done
+   
+(**r NEG64 *)
+      subgoal for x1
+        apply (unfold disassemble_one_instruction_def, auto)
+        done  
 
+(**r HOR64_IMM *)
+      subgoal for x1 x2
+        apply (unfold disassemble_one_instruction_def, auto)
+        done
 
-subgoal for x31 x32 x33 x34
+(**r PRQ + LD_IMM *)
+      subgoal for x1 x2 x3
+        apply (cases x3, auto)
+        apply (unfold insn_def, cases x1, auto)
+        apply (cases x1, auto)
+        done
 
-apply (cases "bpf_ireg2i64 x32 <s 0 \<or> 0xA <s bpf_ireg2i64 x32")
-apply auto
+(**r PQR - LD_IMM *)
+      subgoal for x1 x2 x3
+        apply (cases x3, auto)
+        subgoal for x1'
+          apply (cases x1, auto simp add: insn_def disassemble_one_instruction_def)
+          done
+        subgoal for xa
+          by (cases x1, auto simp add: insn_def disassemble_one_instruction_def)
+        done
 
-apply (cases "snd_op2i64 x33 <s 0 \<or> 0xA <s snd_op2i64 x33")
-apply auto
+(**r PQR64 + LD_IMM *)
+      subgoal for x1 x2 x3
+        apply (cases x3, auto)
+        apply (unfold insn_def, cases x1, auto)
+        apply (cases x1, auto)
+        done  
 
-apply (cases "SCAST(16 signed \<rightarrow> 64 signed) x34 <s 0xFFFFFFFFFFFF8000 \<or> 0x7FFF <s SCAST(16 signed \<rightarrow> 64 signed) x34")
-apply auto
+(**r PQR64 - LD_IMM *)
+      subgoal for x1 x2 x3
+        apply (cases x3, auto)
+        subgoal for x1'
+          apply (cases x1, auto simp add: insn_def disassemble_one_instruction_def)
+          done
+        subgoal for xa
+          apply (cases x1, auto simp add: insn_def disassemble_one_instruction_def)
+          done
+        done  
 
-apply (unfold disassemble_lddw_def)
-apply (cases x31, auto, cases x33, auto)
-apply (cases x33, auto)
-apply (cases x33, auto)
-apply (cases x33, auto)
-.
+(**r PQR2 + LD_IMM *)  
+      subgoal for x1 x2 x3
+        apply (cases x3, auto)
+        apply (unfold insn_def, cases x1, auto)
+        apply (cases x1, auto)
+        done  
 
-subgoal for x31 x32 x33 x34
+(**r PQR2 - LD_IMM *)
+      subgoal for x1 x2 x3
+        apply (cases x3, auto)
+        subgoal for x1'
+          apply (cases x1, auto simp add: insn_def disassemble_one_instruction_def)
+          done
+        subgoal for xa
+          apply (cases x1, auto simp add: insn_def disassemble_one_instruction_def)
+          done
+        done
+ 
+(**r JA *)
+      subgoal for x1
+        apply (unfold insn_def disassemble_one_instruction_def, auto)
+        done
 
-apply (cases "bpf_ireg2i64 x32 <s 0 \<or> 0xA <s bpf_ireg2i64 x32")
-apply auto
+(**r JUMP + LD_IMM  *)
+      subgoal for x1 x2 x3 x4
+        apply (cases x3, auto)
+        apply (unfold insn_def, cases x1, auto)
+        apply (cases x1, auto)
+        done
 
-apply (cases "snd_op2i64 x33 <s 0 \<or> 0xA <s snd_op2i64 x33")
-apply auto
+(**r JUMP - LD_IMM *)
+      subgoal for x1 x2 x3 x4
+        apply (cases x3, auto)
+        subgoal for x1'
+          apply (cases x1, auto simp add: insn_def disassemble_one_instruction_def)
+          done
+        subgoal for x1'
+          apply (cases x1, auto simp add: insn_def disassemble_one_instruction_def)
+          done
+        done
 
-apply (cases "SCAST(16 signed \<rightarrow> 64 signed) x34 <s 0xFFFFFFFFFFFF8000 \<or> 0x7FFF <s SCAST(16 signed \<rightarrow> 64 signed) x34")
-apply auto
+(**r CALL_REG  *)
+      subgoal for x1 x2
+        apply (unfold insn_def disassemble_one_instruction_def, auto)
+        done
 
-apply (cases x31, auto)
-subgoal
-apply (cases x33, auto)
+(**r CALL_IMM  *)
+      subgoal for x1 x2
+        apply (unfold insn_def disassemble_one_instruction_def, auto)
+        done
 
-apply (unfold disassemble_one_instruction_def, auto)
-.
-
-subgoal for x1
-
-apply (cases "0xA < bpf_ireg2i64 x1")
-apply auto
-.    
-
-subgoal for x1
-
-apply (cases "0xA < bpf_ireg2i64 x1")
-apply auto
-.
-
-subgoal for x31 x32
-
-apply (cases "0xA < bpf_ireg2i64 x31")
-apply auto
-.
-
-subgoal for x31 x32 x33
-
-apply (cases "0xA < bpf_ireg2i64 x32")
-apply auto
-apply (cases "0xA < snd_op2i64 x33")
-apply auto
-.   
-
-subgoal for x31
-
-apply (cases "0xA < bpf_ireg2i64 x31")
-apply auto
-.  
-
-subgoal for x31
-
-apply (cases "0xA < bpf_ireg2i64 x31")
-apply auto
-.  
-
-subgoal for x31 x32 x33
-
-apply (cases "0xA < bpf_ireg2i64 x32")
-apply auto
-apply (cases "0xA < snd_op2i64 x33")
-apply auto
-.  
-
-subgoal for x31 x32 x33
-
-apply (cases "0xA < bpf_ireg2i64 x32")
-apply auto
-apply (cases "0xA < snd_op2i64 x33")
-apply auto
-.  
-
-subgoal for x31 x32 x33
-
-apply (cases "0xA < bpf_ireg2i64 x32")
-apply auto
-apply (cases "0xA < snd_op2i64 x33")
-apply auto
-.  
-
-subgoal for x31
-
-apply (cases "SCAST(16 signed \<rightarrow> 64 signed) x31 < 0xFFFFFFFFFFFF8000 \<or>
-        0x7FFF < SCAST(16 signed \<rightarrow> 64 signed) x31")
-apply auto
-.  
-
-subgoal for x1 x2 x3 x4
-
-apply (cases "0xA < bpf_ireg2i64 x2")
-apply auto
-apply (cases "0xA < snd_op2i64 x3")
-apply auto
-
-apply (cases "SCAST(16 signed \<rightarrow> 64 signed) x4 < 0xFFFFFFFFFFFF8000 \<or>
-        0x7FFF < SCAST(16 signed \<rightarrow> 64 signed) x4")
-apply auto
-.  
-
-subgoal for x1 x2
-
-apply (cases "0xA < bpf_ireg2i64 x1")
-apply auto
-.  
-
-subgoal for x1 x2
-
-apply (cases "0xA < bpf_ireg2i64 x1")
-apply auto
-. 
+(**r EXIT *)
+      apply (unfold disassemble_one_instruction_def, auto)
+      done  
+    done
+  done
 
 (**
 apply (induction l_asm arbitrary: l_bin)
@@ -377,27 +419,12 @@ apply (auto simp add: insn_def)
 
 apply (subst aaa(2)[symmetric]) *)
 
-.
-done
 
 (**TODO: consistency between assemble and disassemble *)
 
 
 lemma "(if (0::u64) < 0 \<or> (10::u64) < 0 then None else Some True) = Some True" 
-by fastforce
-
-lemma "bpf_opc x1 = 0x18 \<Longrightarrow>
-       l_bin = a # l_a \<Longrightarrow>
-       bpf_opc a = 0 \<Longrightarrow>
-       bpf_dst a = 0 \<Longrightarrow>
-       bpf_src a = 0 \<Longrightarrow>
-       u4_to_bpf_ireg (bpf_dst x1) = Some aa \<Longrightarrow>
-       disassemble l_a = Some aaa \<Longrightarrow>
-       insn 0x18 0 0 0
-              0 = None"
-              apply (unfold insn_def)
-              apply auto
-              done
+  by fastforce
 (** WHY ?
 
 value "(0::64 sword) < - 0x8000" *)
@@ -409,16 +436,13 @@ value "(0:: i64)"
 value "(0::64 sword) <s ((- 0x8000) :: i64)" *)
 
 lemma disassemble_lddw_assemble_one_instruction[simp]:
-"bpf_opc a = 0x18 \<Longrightarrow> disassemble_lddw (bpf_dst a) (bpf_imm a) aa = Some x1 \<Longrightarrow>
-assemble_one_instruction x1 = Some a"
-apply (unfold disassemble_lddw_def)
-apply (cases "bpf_opc aa = 0 \<and> bpf_dst aa = 0 \<and> bpf_src aa = 0")
-apply auto
-apply (cases "u4_to_bpf_ireg (bpf_dst a)")
-apply auto
-apply (unfold insn_def) 
-
-sorry
+  "bpf_opc a = 0x18 \<Longrightarrow> disassemble_lddw (bpf_dst a) (bpf_imm a) aa = Some x1 \<Longrightarrow>
+  assemble_one_instruction x1 = Some a"
+  apply (unfold disassemble_lddw_def)
+  apply (cases "bpf_opc aa = 0 \<and> bpf_dst aa = 0 \<and> bpf_src aa = 0 \<and> bpf_off aa = 0", auto)
+  apply (cases "u4_to_bpf_ireg (bpf_dst a)", auto)
+  apply (unfold insn_def)
+  sorry
 
 lemma disassemble_lddw_some[simp]:
 "bpf_opc a = 0x18 \<Longrightarrow>
@@ -426,71 +450,58 @@ u4_to_bpf_ireg (bpf_dst a) = Some d \<Longrightarrow>
 disassemble_lddw (bpf_dst a) (bpf_imm a) aa = Some x \<Longrightarrow>
 x = BPF_LD_IMM d (bpf_imm a) (bpf_imm aa)"
 apply (unfold disassemble_lddw_def)
-apply (cases "bpf_opc aa = 0 \<and> bpf_dst aa = 0 \<and> bpf_src aa = 0")
+apply (cases "bpf_opc aa = 0 \<and> bpf_dst aa = 0 \<and> bpf_src aa = 0 \<and> bpf_off aa = 0")
 apply auto
 done
 
+term bpf_opc
 
 lemma disassemble_assemble_consistency: "disassemble l_bin = Some l_asm \<Longrightarrow> assemble l_asm = Some l_bin"
-apply (induction l_asm arbitrary: l_bin)
+  apply (induction l_asm arbitrary: l_bin)
 
 (**r l_asm = [] *)
-subgoal for l_bin
-apply (cases l_bin)
-apply auto
+  subgoal for l_bin
+    apply (cases l_bin, auto)
 
-subgoal for a l_a
-apply (cases "bpf_opc a = 0x18")
-apply auto
+    subgoal for a l_a
+      apply (cases "bpf_opc a = 0x18", auto)
 
-subgoal
-apply (cases l_a)
-apply auto
+      subgoal
+        apply (cases l_a, auto)
 
-subgoal for aa l_aa
-apply (cases "disassemble_lddw (bpf_dst a) (bpf_imm a) aa")
-apply auto
+        subgoal for aa l_aa
+          apply (cases "disassemble_lddw (bpf_dst a) (bpf_imm a) aa", auto)
 
-apply (cases "disassemble l_aa")
-apply auto
-.
-.
+          apply (cases "disassemble l_aa", auto)
+          done
+        done
+      done
 
-apply (cases "disassemble_one_instruction a")
-apply auto
+    subgoal for a l_a
+      apply (cases "disassemble_one_instruction a", auto)
+      apply (cases "disassemble l_a", auto)
+      done
+    done
 
-apply (cases "disassemble l_a")
-apply auto
-.
-.
+(**r l_asm = x1 + l_asm *)
+  subgoal for x1 l_asm l_bin
+    apply (cases l_bin, auto)
 
-subgoal for x1 l_asm l_bin
-apply (cases l_bin)
-apply auto
+    subgoal for a l_a
+      apply (cases "bpf_opc a = 0x18", auto)
 
-subgoal for a l_a
-apply (cases "bpf_opc a = 0x18")
-apply auto
+      subgoal
+        apply (cases l_a, auto)
 
-subgoal
-apply (cases l_a)
-apply auto
-
-subgoal for aa l_aa
-apply (cases "disassemble_lddw (bpf_dst a) (bpf_imm a) aa")
-apply auto
-
-apply (cases "disassemble l_aa")
-apply auto
-
-apply (unfold disassemble_lddw_def)
-apply (cases "bpf_opc aa = 0 \<and> bpf_dst aa = 0 \<and> bpf_src aa = 0")
-apply auto
-
-apply (cases "u4_to_bpf_ireg (bpf_dst a)")
-apply auto
-
-../..
+        subgoal for aa l_aa
+          apply (cases "disassemble_lddw (bpf_dst a) (bpf_imm a) aa", auto)
+          apply (cases "disassemble l_aa", auto)
+          apply (unfold disassemble_lddw_def)
+          apply (cases "bpf_opc aa = 0 \<and> bpf_dst aa = 0 \<and> bpf_src aa = 0", auto)
+          apply (cases "u4_to_bpf_ireg (bpf_dst a)", auto)
+          apply (unfold insn_def, auto)
+          done
+../.. TBC
 apply (unfold insn_def)
 apply auto
 .
@@ -570,6 +581,7 @@ apply auto
 subgoal
 
 .
+declare if_split_asm [split del] (**r remove this config*)
 
 done
 end
