README.md
@@ -7,20 +7,26 @@
 - [ ] _More: formalize rbpf's verifier, static analysis, memory model, and JIT compiler (correctness proof) ..._
 
 # How to install
-- [Isabelle/HOL 2023](https://isabelle.in.tum.de/) (please set your PATH with e.g. `/YOUR-PATH/Isabelle2023`)
-- [AutoCorres 1.10](https://github.com/seL4/l4v/releases/tag/autocorres-1.10)
+- [Isabelle/HOL 2024](https://isabelle.in.tum.de/) (please set your PATH with e.g. `/YOUR-PATH/Isabelle2024`)
+
+- [Isabelle AFP](https://www.isa-afp.org/download/)
 
 ```shell
-# 1. assume the current folder is the root of CertSBF
-# 2. assume you has downloaded Isabelle2023 and autocorres
 
-# unzip autocorres on the folder of the Isabelle/HOL home folder
-tar -zxvf YOUR-AUTOCORRES-DIR/autocorres-1.10.tar.gz -C /YOUR-PATH/Isabelle2023/
+# set PATH 
+cd ~
+vim. bashrc # export PATH=$PATH:/PATH/Isabelle2024/bin:...
+source .bashrc
 
-# confige info
-./configure --isabelledir=/YOUR-PATH/Isabelle2023
+# test isabelle/hol
+isabelle version # Isabelle2024
 
-# open Isabelle/HOL with autocorres
+# config AFP
+cd /YOUR-PATH/afp/thys
+isabelle components -u .
+
+# go to CertSBF folder and open this project in jedit
+cd /YOUR-PATH/CertSBF
 make
 ```
 
